Foundation/InterpretabilityLogic/Entailment.lean
@@ -1,41 +1,43 @@
 import Foundation.InterpretabilityLogic.Entailment.IL
 import Foundation.InterpretabilityLogic.Entailment.IL_KW1Zero
 import Foundation.InterpretabilityLogic.Entailment.IL_KW2
-import Foundation.InterpretabilityLogic.Entailment.ILM
-import Foundation.InterpretabilityLogic.Entailment.ILM₀.Basic
+import Foundation.InterpretabilityLogic.Entailment.IL_M
+import Foundation.InterpretabilityLogic.Entailment.IL_M₀_W
+import Foundation.InterpretabilityLogic.Entailment.IL_M₀
+import Foundation.InterpretabilityLogic.Entailment.IL_P
+import Foundation.InterpretabilityLogic.Entailment.IL_R
+import Foundation.InterpretabilityLogic.Entailment.IL_R_W
+import Foundation.InterpretabilityLogic.Entailment.IL_Rstar
+import Foundation.InterpretabilityLogic.Entailment.IL_W
+import Foundation.InterpretabilityLogic.Entailment.IL_Wstar
 import Foundation.InterpretabilityLogic.Entailment.ILMinus
 import Foundation.InterpretabilityLogic.Entailment.ILMinus_J1
 import Foundation.InterpretabilityLogic.Entailment.ILMinus_J2
 import Foundation.InterpretabilityLogic.Entailment.ILMinus_J4
 import Foundation.InterpretabilityLogic.Entailment.ILMinus_J5
 import Foundation.InterpretabilityLogic.Entailment.ILMinus_M
-import Foundation.InterpretabilityLogic.Entailment.ILP
-import Foundation.InterpretabilityLogic.Entailment.ILR
-import Foundation.InterpretabilityLogic.Entailment.ILRStar
-import Foundation.InterpretabilityLogic.Entailment.ILRW
-import Foundation.InterpretabilityLogic.Entailment.ILW
-import Foundation.InterpretabilityLogic.Entailment.ILWM₀
-import Foundation.InterpretabilityLogic.Entailment.ILWStar.Basic
-import Foundation.InterpretabilityLogic.Entailment.ILWStar.M₀
 
 namespace LO.InterpretabilityLogic.Entailment
 
 variable {S F : Type*} [DecidableEq F] [InterpretabilityLogicalConnective F] [Entailment S F] {𝓢 : S}
 
-instance [Entailment.ILWM₀ 𝓢] : Entailment.ILWStar 𝓢 where
+instance [Entailment.IL_M₀_W 𝓢] : Entailment.IL_Wstar 𝓢 where
 
-instance [Entailment.ILM 𝓢] : Entailment.ILRW 𝓢 where
-instance [Entailment.ILW 𝓢] : Entailment.IL_KW2 𝓢 where
-instance [Entailment.ILW 𝓢] : Entailment.HasAxiomF 𝓢 := «IL(KW2)_⊢_F»
+instance [Entailment.IL_M 𝓢] : Entailment.IL_R_W 𝓢 where
+instance [Entailment.IL_W 𝓢] : Entailment.IL_KW2 𝓢 where
+instance [Entailment.IL_W 𝓢] : Entailment.HasAxiomF 𝓢 := «IL(KW2)_⊢_F»
 
-instance [Entailment.ILM 𝓢] : Entailment.ILRStar 𝓢 where
-instance [Entailment.ILM 𝓢] : Entailment.ILW 𝓢 where
-instance [Entailment.ILM 𝓢] : Entailment.ILR 𝓢 where
-instance [Entailment.ILM 𝓢] : Entailment.ILRW 𝓢 where
+instance [Entailment.IL_M 𝓢] : Entailment.IL_Rstar 𝓢 where
+instance [Entailment.IL_M 𝓢] : Entailment.IL_W 𝓢 where
+instance [Entailment.IL_M 𝓢] : Entailment.IL_R 𝓢 where
+instance [Entailment.IL_M 𝓢] : Entailment.IL_R_W 𝓢 where
 
-instance [Entailment.ILP 𝓢] : Entailment.ILW 𝓢 where
-instance [Entailment.ILP 𝓢] : Entailment.ILR 𝓢 where
-instance [Entailment.ILP 𝓢] : Entailment.ILRW 𝓢 where
-instance [Entailment.ILP 𝓢] : Entailment.ILRStar 𝓢 where
+instance [Entailment.IL_P 𝓢] : Entailment.IL_W 𝓢 where
+instance [Entailment.IL_P 𝓢] : Entailment.IL_R 𝓢 where
+instance [Entailment.IL_P 𝓢] : Entailment.IL_R_W 𝓢 where
+instance [Entailment.IL_P 𝓢] : Entailment.IL_Rstar 𝓢 where
+
+instance [Entailment.IL_Wstar 𝓢] : Entailment.IL_W 𝓢 where
+instance [Entailment.IL_Wstar 𝓢] : Entailment.IL_M₀ 𝓢 where
 
 end LO.InterpretabilityLogic.Entailment
