Foundation/InterpretabilityLogic/Veltman/Logic/IL_P.lean
@@ -1,5 +1,6 @@
-import Foundation.InterpretabilityLogic.Veltman.Logic.ILRW
-import Foundation.InterpretabilityLogic.Veltman.AxiomM
+import Foundation.InterpretabilityLogic.Veltman.Logic.IL
+import Foundation.InterpretabilityLogic.Veltman.AxiomP
+import Foundation.InterpretabilityLogic.Veltman.Logic.IL_R_W
 
 namespace LO.InterpretabilityLogic
 
@@ -8,35 +9,35 @@ open Veltman
 
 namespace Veltman
 
-protected class Frame.IsILM (F : Veltman.Frame) extends F.IsIL, F.HasAxiomM
-protected abbrev FrameClass.ILM : FrameClass := { F | F.IsILM }
+protected class Frame.IsIL_P (F : Veltman.Frame) extends F.IsIL, F.HasAxiomP
+protected abbrev FrameClass.IL_P : FrameClass := { F | F.IsIL_P }
 
-instance : trivialFrame.IsILM where
-  S_M := by tauto
+instance : trivialFrame.IsIL_P where
+  S_P := by tauto
 
 end Veltman
 
 
 open Hilbert.Basic
 
-namespace ILM
+namespace IL_P
 
-instance Veltman.sound : Sound InterpretabilityLogic.ILM FrameClass.ILM := by
+instance Veltman.sound : Sound InterpretabilityLogic.IL_P FrameClass.IL_P := by
   apply Veltman.instFrameClassSound;
   constructor;
   intro φ hφ F hF;
   replace hF := Set.mem_setOf_eq.mp hF;
   rcases hφ with (rfl | rfl | rfl | rfl | rfl | rfl) <;> simp;
 
-instance : Entailment.Consistent InterpretabilityLogic.ILM := Veltman.consistent_of_sound_frameclass FrameClass.ILM $ by
+instance : Entailment.Consistent InterpretabilityLogic.IL_P := Veltman.consistent_of_sound_frameclass FrameClass.IL_P $ by
   use Veltman.trivialFrame;
   apply Set.mem_setOf_eq.mpr;
   infer_instance;
 
-end ILM
+end IL_P
 
 open Entailment in
-instance : InterpretabilityLogic.ILRW ⪱ InterpretabilityLogic.ILM := by
+instance : InterpretabilityLogic.IL_R_W ⪱ InterpretabilityLogic.IL_P := by
   constructor;
   . apply weakerThan_of_provable_axioms;
     intro φ hφ;
@@ -44,23 +45,21 @@ instance : InterpretabilityLogic.ILRW ⪱ InterpretabilityLogic.ILM := by
       axiomJ1, axiomJ2, axiomJ3, axiomJ4, axiomJ5, axiomR, axiomW,
     ];
   . apply Entailment.not_weakerThan_iff.mpr;
-    use (Axioms.M (.atom 0) (.atom 1) (.atom 2));
+    use (Axioms.P (.atom 0) (.atom 1));
     constructor;
     . simp;
-    . apply Sound.not_provable_of_countermodel (𝓜 := Veltman.FrameClass.ILRW);
+    . apply Sound.not_provable_of_countermodel (𝓜 := Veltman.FrameClass.IL_R_W);
       apply Veltman.not_validOnFrameClass_of_exists_frame;
       use {
         toKripkeFrame := {
           World := Fin 4
-          Rel x y := (x = 0 ∧ 0 < y) ∨ (x = 2 ∧ y = 3)
+          Rel x y := (x = 0 ∧ 0 < y) ∨ (x = 1 ∧ y = 2)
         }
         isGL := Modal.Kripke.Frame.isGL_of_isFiniteGL {
           trans := by omega;
           irrefl := by omega;
         }
-        S w x y :=
-           (w = 0 ∧ 1 ≤ x ∧ x ≤ y) ∨
-           (w = 2 ∧ x = 3 ∧ y = 3)
+        S w x y := (w = 0 ∧ 1 ≤ x ∧ x ≤ y) ∨ (w = 1 ∧ x = 2 ∧ y = 2)
         S_cond := by grind;
       }
       constructor;
@@ -70,7 +69,6 @@ instance : InterpretabilityLogic.ILRW ⪱ InterpretabilityLogic.ILM := by
           S_J2 := by grind;
           S_J4 := by grind;
           S_J5 := by grind;
-          S_R := by grind;
           S_W {w} := by
             apply Finite.converseWellFounded_of_trans_irrefl';
             . infer_instance
@@ -80,9 +78,10 @@ instance : InterpretabilityLogic.ILRW ⪱ InterpretabilityLogic.ILM := by
             . dsimp [Irreflexive, Frame.RS, Relation.Comp];
               push_neg;
               grind;
+          S_R := by grind;
         }
       . by_contra hC;
-        have := Veltman.Frame.HasAxiomM.of_validate_axiomM hC |>.S_M (w := 0) (x := 1) (y := 2) (z := 3) (by tauto) (by tauto);
+        have := Veltman.Frame.HasAxiomP.of_validate_axiomP hC |>.S_P (w := 0) (x := 1) (y := 2) (z := 3) (by tauto) (by tauto);
         contradiction;
 
 end LO.InterpretabilityLogic
