Foundation/InterpretabilityLogic/Veltman/Logic/IL_P₀.lean
@@ -8,35 +8,35 @@ open Veltman
 
 namespace Veltman
 
-protected class Frame.IsILP₀ (F : Veltman.Frame) extends F.IsIL, F.HasAxiomR
-protected abbrev FrameClass.ILP₀ : FrameClass := { F | F.IsILP₀ }
+protected class Frame.IsIL_P₀ (F : Veltman.Frame) extends F.IsIL, F.HasAxiomR
+protected abbrev FrameClass.IL_P₀ : FrameClass := { F | F.IsIL_P₀ }
 
 instance : trivialFrame.HasAxiomR where
   S_R := by tauto;
-instance : trivialFrame.IsILP₀ where
+instance : trivialFrame.IsIL_P₀ where
 
 end Veltman
 
 
 open Hilbert.Basic
 
-namespace ILP₀
+namespace IL_P₀
 
-instance Veltman.sound : Sound InterpretabilityLogic.ILP₀ FrameClass.ILP₀ := by
+instance Veltman.sound : Sound InterpretabilityLogic.IL_P₀ FrameClass.IL_P₀ := by
   apply Veltman.instFrameClassSound;
   constructor;
   intro φ hφ F hF;
   replace hF := Set.mem_setOf_eq.mp hF;
   rcases hφ with (rfl | rfl | rfl | rfl | rfl | rfl) <;> simp;
 
-instance : Entailment.Consistent InterpretabilityLogic.ILP₀ := Veltman.consistent_of_sound_frameclass FrameClass.ILP₀ $ by
+instance : Entailment.Consistent InterpretabilityLogic.IL_P₀ := Veltman.consistent_of_sound_frameclass FrameClass.IL_P₀ $ by
   use Veltman.trivialFrame;
   apply Set.mem_setOf_eq.mpr;
   infer_instance;
 
-end ILP₀
+end IL_P₀
 
-instance : InterpretabilityLogic.IL ⪱ InterpretabilityLogic.ILP₀ := by
+instance : InterpretabilityLogic.IL ⪱ InterpretabilityLogic.IL_P₀ := by
   constructor;
   . apply weakerThan_of_subset_axioms $ by grind;
   . apply Entailment.not_weakerThan_iff.mpr;
