Foundation/InterpretabilityLogic/Veltman/Logic/IL_R_W.lean
@@ -1,6 +1,6 @@
-import Foundation.InterpretabilityLogic.Veltman.Logic.ILR
-import Foundation.InterpretabilityLogic.Veltman.Logic.ILW
-import Foundation.InterpretabilityLogic.Veltman.Logic.ILWM₀
+import Foundation.InterpretabilityLogic.Veltman.Logic.IL_R
+import Foundation.InterpretabilityLogic.Veltman.Logic.IL_W
+import Foundation.InterpretabilityLogic.Veltman.Logic.IL_M₀_W
 
 namespace LO.InterpretabilityLogic
 
@@ -9,19 +9,19 @@ open Veltman
 
 namespace Veltman
 
-protected class Frame.IsILRW (F : Veltman.Frame) extends F.IsIL, F.HasAxiomW, F.HasAxiomR
-protected abbrev FrameClass.ILRW : FrameClass := { F | F.IsILRW }
+protected class Frame.IsIL_R_W (F : Veltman.Frame) extends F.IsIL, F.HasAxiomW, F.HasAxiomR
+protected abbrev FrameClass.IL_R_W : FrameClass := { F | F.IsIL_R_W }
 
-instance : trivialFrame.IsILRW where
+instance : trivialFrame.IsIL_R_W where
 
 end Veltman
 
 
 open Hilbert.Basic
 
-namespace ILRW
+namespace IL_R_W
 
-instance Veltman.sound : Sound InterpretabilityLogic.ILRW FrameClass.ILRW := by
+instance Veltman.sound : Sound InterpretabilityLogic.IL_R_W FrameClass.IL_R_W := by
   apply Veltman.instFrameClassSound;
   constructor;
   intro φ hφ F hF;
@@ -29,15 +29,15 @@ instance Veltman.sound : Sound InterpretabilityLogic.ILRW FrameClass.ILRW := by
   replace hF := Set.mem_setOf_eq.mp hF;
   rcases hφ with (rfl | rfl | rfl | rfl | rfl | rfl | rfl) <;> simp;
 
-instance : Entailment.Consistent InterpretabilityLogic.ILRW := Veltman.consistent_of_sound_frameclass FrameClass.ILRW $ by
+instance : Entailment.Consistent InterpretabilityLogic.IL_R_W := Veltman.consistent_of_sound_frameclass FrameClass.IL_R_W $ by
   use Veltman.trivialFrame;
   apply Set.mem_setOf_eq.mpr;
   infer_instance;
 
-end ILRW
+end IL_R_W
 
 open Entailment in
-instance : InterpretabilityLogic.ILWM₀ ⪱ InterpretabilityLogic.ILRW := by
+instance : InterpretabilityLogic.IL_M₀_W ⪱ InterpretabilityLogic.IL_R_W := by
   constructor;
   . apply weakerThan_of_provable_axioms;
     intro φ hφ;
@@ -48,7 +48,7 @@ instance : InterpretabilityLogic.ILWM₀ ⪱ InterpretabilityLogic.ILRW := by
     use (Axioms.R (.atom 0) (.atom 1) (.atom 2));
     constructor;
     . simp;
-    . apply Sound.not_provable_of_countermodel (𝓜 := Veltman.FrameClass.ILWM₀);
+    . apply Sound.not_provable_of_countermodel (𝓜 := Veltman.FrameClass.IL_M₀_W);
       apply Veltman.not_validOnFrameClass_of_exists_frame;
       let F : Veltman.Frame := {
         toKripkeFrame := ⟨Fin 5, λ x y => (x = 0 ∧ 0 < y) ∨ (x = 1 ∧ (y = 2 ∨ y = 4)) ∨ (x = 3 ∧ y = 4)⟩
@@ -62,7 +62,7 @@ instance : InterpretabilityLogic.ILWM₀ ⪱ InterpretabilityLogic.ILRW := by
           (w = 3 ∧ x = 4 ∧ y = 4)
         S_cond := by grind;
       }
-      have : F.IsILWM₀ := {
+      have : F.IsIL_M₀_W := {
         S_J1 := by grind;
         S_J2 := by grind;
         S_J4 := by grind;
@@ -89,14 +89,14 @@ instance : InterpretabilityLogic.ILWM₀ ⪱ InterpretabilityLogic.ILRW := by
         have : F.SRel' 1 2 4 := Frame.HasAxiomR.of_validate_axiomR hC |>.S_R (x := 0) (u := 3) (by tauto) (by tauto) (by tauto) (by tauto);
         simp [F, Frame.SRel'] at this;
 
-instance «ILR ⪱ ILRW» : InterpretabilityLogic.ILR ⪱ InterpretabilityLogic.ILRW := by
+instance «IL_R ⪱ IL_R_W» : InterpretabilityLogic.IL_R ⪱ InterpretabilityLogic.IL_R_W := by
   constructor;
   . apply weakerThan_of_subset_axioms $ by grind;
   . apply Entailment.not_weakerThan_iff.mpr;
     use (Axioms.W (.atom 0) (.atom 1));
     constructor;
     . simp;
-    . apply Sound.not_provable_of_countermodel (𝓜 := Veltman.FrameClass.ILR);
+    . apply Sound.not_provable_of_countermodel (𝓜 := Veltman.FrameClass.IL_R);
       apply Veltman.not_validOnFrameClass_of_exists_frame;
       let F : Veltman.Frame := {
         toKripkeFrame := ⟨Fin 3, (· < ·)⟩
@@ -107,7 +107,7 @@ instance «ILR ⪱ ILRW» : InterpretabilityLogic.ILR ⪱ InterpretabilityLogic.
         S w x y := (w = 0 ∧ x ≠ 0 ∧ y ≠ 0) ∨ (w = 1 ∧ x = 2 ∧ y = 2)
         S_cond := by grind;
       }
-      have : F.IsILR := {
+      have : F.IsIL_R := {
         S_J1 := by dsimp [Frame.SRel', F]; omega;
         S_J2 := by dsimp [Frame.SRel', F]; omega;
         S_J4 := by dsimp [Frame.SRel', F]; omega;
